Naturals Model compiler

src/named/BedrockModel.v
@@ -2,17 +2,17 @@ Set Implicit Arguments.
 Set Bullet Behavior "Strict Subproofs".
 
 Require Import String List.
+Require Import Numbers.DecimalNat Numbers.DecimalString.
 Require Vector.
 Import ListNotations.
 Open Scope string.
 Open Scope list.
 
-From bedrock2 Require Import Syntax.
+From bedrock2 Require Import Syntax Semantics.
 
 From Utils Require Import Utils.
-From Named Require Import Substable Model GeneralModel.
-From Named Require Import Term Rule.
-
+From Named Require Import Substable Model GeneralModel Term Rule Core CompilerDefs.
+Import Core.Notations.
 
 
 Notation named_list := (@named_list string).
@@ -23,6 +23,21 @@ Notation sort := (@sort string).
 Notation subst := (@subst string).
 Notation rule := (@rule string).
 Notation lang := (@lang string).
+Print exec.exec.
+Context (width : BinNums.Z)
+        (word : Interface.word.word width)
+        (key := Interface.word.rep (width := width))
+        (value := Init.Byte.byte : Type)
+        (mem : Interface.map.map key value)
+        (locals : Interface.map.map string (Interface.word.rep (width := width)))
+        (env : Interface.map.map string (list string * list string * cmd))
+        (m : Interface.map.rep (key := key) (value := value) (map := mem))
+        (l : Interface.map.rep (key := string) (value := key) (map := locals))
+        (BW : Bitwidth.Bitwidth width)
+        (ext_spec : ExtSpec)
+        (e : Interface.map.rep (key := string) (value := list string * list string * cmd) (map := env)).
+
+
 
 (* This the the `term` type that should get plugged into the general model.
    We'll be adding a few more sorts later, but this is good for now.
@@ -41,31 +56,292 @@ Notation lang := (@lang string).
  *)
 
 (* this *)
-Variant bedrock_term :=
+Variant bedrock_exp :=
   | bedrock_expr (e : expr)
-  | bedrock_cmd (c : cmd).
+  | bedrock_cmd (c : cmd)
+  | bedrock_nat (n : nat).
 
-Variant bedrock_sort :=
-  | br_expr
-  | br_cmd.
+(* Variant br_expr : Set := *)
+(*   | br_expr_tt. *)
+(* Variant br_cmd : Set := *)
+(*   | br_cmd_tt. *)
+(* Variant br_nat : Set := *)
+(*   | br_nat_tt. *)
 
-Print Substable0.
-Print Model.Model.
+(* Variant bedrock_sort := *)
+(*   | br_expr_srt *)
+(*   | br_cmd_srt *)
+(*   | br_nat_srt. *)
 
-Print Model.Model_ok.
-Print Substable.subst.
-Set Printing Implicit.
-Print GeneralModel.model.
 
-Check (GeneralModel.model (V := string)).
 
-(* Need to supply eq_sort, eq_term, wf_sort, wf_term on lcosed terms here *)
-Definition bedrock_model := GeneralModel.model (V := string) bedrock_term.
-Definition bedrock_model_ok : Model.Model_ok bedrock_model := GeneralModel.model_ok bedrock_term bedrock_sort.
+Notation bedrock_term := (GeneralModel.term (V := string) bedrock_exp).
 
-Check GeneralModel.model.
-Check Model.Model.
-Check bedrock_model.
+(* This is just a copy of the lang in NatLang.v, temporarily
+   placed here while Elab and a few other files are broken. *)
+Definition nat_lang_def : lang := 
+  {[l
+  [s|
+      -----------------------------------------------
+      #"natural" srt
+  ];
+  [:|  
+       -----------------------------------------------
+       #"0" : #"natural"
+  ];
+  [:|  "n": #"natural"
+       -----------------------------------------------
+       #"1+" "n" : #"natural"
+  ];
+  [:|
+       "a" : #"natural",
+       "b" : #"natural" 
+       -----------------------------------------------
+       #"plus" "a" "b" : #"natural"
+  ]
+  (* [:= *)
+  (*      "a" : #"natural" *)
+  (*      ----------------------------------------------- ("plus_0") *)
+  (*      #"plus" "a" #"0" = "a" : #"natural" *)
+  (* ]; *)
+  (* [:= *)
+  (*      "a" : #"natural", *)
+  (*      "b" : #"natural" *)
+  (*      ----------------------------------------------- ("plus_1+") *)
+  (*      #"plus" "a" (#"1+" "b") = #"plus" (#"1+" "a") "b" : #"natural" *)
+  (* ] *)
+    ]}.
+
+
+Definition bedrock_subset_def : lang :=
+  {[l
+      [s|
+      -----------------------------------------------
+        #"expr" srt
+      ];
+    [:| "n" : #"natural"
+      -----------------------------------------------
+      #"literal" "n" : #"expr"
+    ];
+    [:| "n" : #"natural"
+      -----------------------------------------------
+      #"var" "n" : #"expr"
+    ];
+    [s|
+      -----------------------------------------------
+      #"cmd" srt
+      ];
+    [:|
+       -----------------------------------------------
+      #"skip" : #"cmd"
+    ];
+    [:|
+        "lhs" : #"natural",
+        "rhs" : #"expr"
+        -----------------------------------------------
+      #"set" "lhs" "rhs" : #"cmd"
+    ];
+    [:|
+        "s1" : #"cmd",
+        "s2" : #"cmd"
+      -----------------------------------------------
+     #"seq" "s1" "s2" : #"cmd"
+    ];
+    [:| "test" : #"expr",
+        "body" : #"cmd"
+      -----------------------------------------------
+      #"while" "test" "body" : #"cmd"
+    ]
+    ]}.
+     (* Add a few (1-2) interesting equalities from the original language *)
+
+
+Local Notation compiler := (compiler string (tgt_term := bedrock_term) (tgt_sort := Type)).
+
+Definition nat_to_string (n : nat) := NilZero.string_of_uint (Decimal.rev (Unsigned.to_lu n)).
+
+Definition default_cmd : bedrock_exp := bedrock_cmd cmd.skip.
+Definition default_expr : bedrock_exp := bedrock_expr (expr.literal BinNums.Z0).
+
+Definition with_nat name ms f : bedrock_exp :=
+  match named_list_lookup default_expr ms name with
+  | bedrock_nat z => f z
+  | _ => default_cmd
+  end.
+
+Definition with_cmd name ms f : bedrock_exp :=
+  match named_list_lookup default_expr ms name with
+  | bedrock_cmd c => f c
+  | _ => default_cmd
+  end.
+
+Definition with_expr name ms f : bedrock_exp :=
+  match named_list_lookup default_cmd ms name with
+  | bedrock_expr e => f e
+  | _ => default_cmd
+  end.
+
+Definition literal_term (n_str : string) : bedrock_term :=
+  fun ms =>
+    with_nat n_str ms (fun n =>
+    bedrock_expr (expr.literal (BinInt.Z.of_nat n))).
+
+Definition var_term n_str : bedrock_term :=
+  fun ms =>
+    with_nat n_str ms (fun n =>
+    bedrock_expr (expr.var (nat_to_string n))).
+
+Definition set_term lhs_str rhs_str : bedrock_term :=
+  fun ms =>
+    with_nat lhs_str ms (fun lhs =>
+    with_expr rhs_str ms (fun rhs =>
+    bedrock_cmd (cmd.set (nat_to_string lhs) rhs))).
+
+Definition seq_term s1_str s2_str : bedrock_term :=
+  fun ms =>
+    with_cmd s1_str ms (fun s1 =>
+    with_cmd s2_str ms (fun s2 =>
+    bedrock_cmd (cmd.seq s1 s2))).
+
+Definition while_term (t_str b_str : string) : bedrock_term :=
+  fun ms =>
+    with_expr t_str ms (fun test =>
+    with_cmd b_str ms (fun body =>
+    bedrock_cmd (cmd.while test body))).
+
+Definition succ_term (n_str : string) : bedrock_term :=
+  fun ms =>
+    with_nat n_str ms (fun n =>
+    bedrock_nat (S n)).
+
+Definition plus_term (a_str b_str : string) : bedrock_term :=
+  fun ms =>
+    with_nat a_str ms (fun a =>
+    with_nat b_str ms (fun b =>
+    bedrock_nat (a + b))).
+
+
+Notation eval_expr_old := (eval_expr_old (width := width) (mem := mem) (locals := locals) m l).
+Notation exec_exec := (exec.exec (width := width) (BW := BW) (word := word) (mem := mem)
+                                 (locals := locals) (env := env) (ext_spec := ext_spec) e).
+
+Definition eq_exp (e1 e2 : bedrock_exp) :=
+  match e1, e2 with
+  | bedrock_expr e1', bedrock_expr e2' => eval_expr_old e1' = eval_expr_old e2'
+  | bedrock_cmd c1, bedrock_cmd c2 => forall tr r1 r2 ml f, exec_exec c1 tr r1 r2 ml f <-> exec_exec c2 tr r1 r2 ml f
+  | bedrock_nat n1, bedrock_nat n2 => n1 = n2
+  | _, _ => False
+  end.
+
+
+Definition wf_exp (e : bedrock_exp) (t : Type) :=
+    match e with
+    | bedrock_cmd _ => t = cmd
+    | bedrock_expr _ => t = expr
+    | bedrock_nat _ => t = nat
+    end.
+
+Lemma exp_refl : forall e, eq_exp e e.
+Proof.
+  intros; destruct e0; unfold eq_exp; try constructor; intros; try trivial.
+Qed.
+
+Lemma exp_trans : forall e1 e2 e3, eq_exp e1 e2 -> eq_exp e2 e3 -> eq_exp e1 e3.
+Proof.
+  intros; destruct e1, e2, e3; unfold eq_exp in *; try contradiction.
+  {rewrite H; trivial.}
+  {constructor; specialize (H tr r1 r2 ml f); specialize (H0 tr r1 r2 ml f); destruct H, H0; intros; trivial.
+   - apply H0; apply H; trivial.
+   - apply H1; apply H2; trivial.
+  }
+  {rewrite H; trivial.}
+Qed.
+
+Lemma exp_symm : forall e1 e2, eq_exp e1 e2 -> eq_exp e2 e1.
+Proof.
+  intros; destruct e1, e2; unfold eq_exp in *; try contradiction; auto.
+  constructor; specialize (H tr r1 r2 ml f); destruct H; trivial.
+Qed.
+
+Definition bedrock_model := GeneralModel.model (exp := bedrock_exp) default_cmd eq_exp wf_exp.
+Definition bedrock_model_ok : Model.Model_ok bedrock_model :=
+  GeneralModel.model_ok default_cmd eq_exp exp_symm exp_trans exp_refl wf_exp.
+
+Definition bedrock_subset_compiler : compiler :=
+  [
+    ("while", term_case ["body"; "test"] (while_term "test" "body"));
+    ("seq", term_case ["s2"; "s1"] (seq_term "s1" "s2"));
+    ("set", term_case ["rhs"; "lhs"] (set_term "lhs" "rhs"));
+    ("skip", term_case [] (fun _ => bedrock_cmd cmd.skip));
+    ("cmd", sort_case [] (cmd : Type));
+    ("var", term_case ["n"] (var_term "n"));
+    ("literal", term_case ["n"] (literal_term "n"));
+    ("expr", sort_case [] (expr : Type));
+    ("plus", term_case ["b"; "a"] (plus_term "a" "b"));
+    ("1+", term_case ["n"] (succ_term "n"));
+    ("0", term_case [] (fun _ => bedrock_nat 0));
+    ("natural", sort_case [] (nat : Type))
+  ].
+
+Definition example1 :=
+  {{e #"seq" (#"while" (#"literal" #"0") (#"set" (#"1+" #"0") (#"literal" (#"1+" (#"1+" #"0"))))) (#"set" #"0" (#"var" #"0"))}}.
+
+Definition example2 :=
+  {{e #"while" (#"literal" #"0") (#"set" #"0" (#"literal" #"0"))}}.
+
+Print compile.
+Notation compile :=
+  (compile (V := string) (V_Eqb := string_Eqb)
+           (tgt_term := bedrock_term) (H := fun _ => default_expr)
+           (tgt_Model := bedrock_model) bedrock_subset_compiler).
+
+Definition compiled_example :=
+  compile example1.
+
+Compute (compiled_example).
+
+Ltac break_preserving_compiler :=
+  unfold bedrock_subset_compiler, bedrock_subset_def, nat_lang_def; simpl;
+  repeat match goal with
+         | [ |- preserving_compiler_ext _ _ ((_, term_rule ?c' _ _) :: _)] =>
+             apply preserving_compiler_term with (c := c')
+         | [ |- preserving_compiler_ext _ _ ((_, sort_rule ?c' _) :: _)] =>
+             apply preserving_compiler_sort with (c := c')
+         | [ |- preserving_compiler_ext _ [] []] =>
+             apply preserving_compiler_nil
+  end.
+
+Ltac bedrock_crush :=
+  unfold Model.wf_sort; simpl;
+  unfold GeneralModel.wf_sort, GeneralModel.wf_term, GeneralModel.ws_term; simpl;
+  try trivial;
+  repeat match goal with
+         | [ |- _ /\ _] => apply conj
+         | [ |- NoDup []] => apply NoDup_nil
+         | [ |- NoDup (_ :: _)] => apply NoDup_cons
+         | [ |- ~ _] => unfold not
+         | _ => idtac
+         end;
+  simpl; try trivial.
+
+Theorem bedrock_compiler_preserving :
+  preserving_compiler_ext (tgt_Model := bedrock_model) (H := fun _ => default_expr)
+                          (H0 := nat) [] bedrock_subset_compiler (bedrock_subset_def ++ nat_lang_def).
+Proof.
+  break_preserving_compiler;
+  bedrock_crush.
+  1: {intros.
+      unfold eq_exp, succ_term, with_nat.
+
+  }
+  
+(*
+  TODO:
+  Describe project in text for other people to look at and understand.
+  REMEMBER TO PUSH!!
+  Prove that you can compile the language without any equalities.
+  Add equations about nats.
+  Add equations about expressions.
+*)
+
 Definition get_substable (m : Model.Model) : Substable.Substable.
-
-  (* Make a pyrosome language with a limited subset of the bedrock language *)
